DPLL/x.lisp
@@ -1,0 +1,47 @@
+(thm
+    (implies
+     ( (lambda (expt_gamma_h expt_gamma_minus_h h)
+		  (implies
+		    (and  (rationalp expt_gamma_minus_h)
+			  (rationalp expt_gamma_h)
+			  (integerp h)
+			  (equal expt_gamma_minus_h (/ expt_gamma_h))
+			  (< '0 expt_gamma_h)
+			  (< expt_gamma_h '1)
+			  (not (< h '1))
+		    )
+		    (<
+		      (+
+			(* expt_gamma_h
+			   ( (lambda (|var0|)
+			       (+ '-1
+				  (* (* '1 (/ (* '1 '1)))
+				     (* (+ '1 (* '1 '1))
+					(/ (+ '1 (* '1 (+ (* |var0| '1/3200) (+ (* (* '1 (/ (* '1 (* '1 '1)))) (+ '1 (* '1 '1))) (- (* '1 (/ '1))))))))
+				     )))
+			     ) h))
+			(* expt_gamma_minus_h
+			   ( (lambda (|var1|)
+			       (+ '-1
+				  (* (* '1 (/ (* '1 '1)))
+				     (* (+ '1 (* '1 '1))
+					(/ (+ '1 (* '1 (+ (* |var1| '1/3200) (+ (* (* '1 (/ (* '1 (* '1 '1)))) (+ '1 (* '1 '1))) (- (* '1 (/ '1))))))))
+				     )))
+			     ) (- h)))
+		    )
+		    '0)
+		  ))
+	   (b-term-expt h) (b-term-expt (- h)) h)
+    (implies
+      (if (integerp h) (not (< h '1)) 'nil)
+      (<
+	(+ (* (b-term-expt h) (b-term-rest h))
+	   (* (b-term-expt (- h)) (b-term-rest (- h))))
+	'0))
+  )
+)
+;; Subgoal 1.3
+(implies (not (integerp h))
+         (< (+ (* 2 (/ (+ 2 (* 1/3200 h))))
+               (* 2 (/ (+ 2 (- (* 1/3200 h))))))
+            2))
