smtlink/test-all.lisp
@@ -25,93 +25,93 @@
 			   (:hypothesize ()))
 			 ))))
 
-;; ;; test1
-;; (defun foo1 (x y) (* x (+ 1 y)))
+;; test1
+(defun foo1 (x y) (* x (+ 1 y)))
 
-;; ;; very first piece of test case
-;; (defthm test1 (implies (and (and (rationalp x)
-;; 				 (integerp y)
-;; 				 (integerp z))
-;; 			    (and (not (<= x 0))
-;; 				 (equal z (+ 3/2 4))
-;; 				 (or (> x y) (> x (+ y 40/3)))))
-;; 		       (> (foo1 x (foo1 x z)) (foo1 x y)))
-;;   :hints
-;;   (("Goal"
-;;     :clause-processor
-;;     (my-clause-processor clause
-;; 			 '( (:expand (foo1))
-;; 			   (:python-file "test1")
-;; 			   (:let ())
-;; 			   (:hypothesize ()))))))
+;; very first piece of test case
+(defthm test1 (implies (and (and (rationalp x)
+				 (integerp y)
+				 (integerp z))
+			    (and (not (<= x 0))
+				 (equal z (+ 3/2 4))
+				 (or (> x y) (> x (+ y 40/3)))))
+		       (> (foo1 x (foo1 x z)) (foo1 x y)))
+  :hints
+  (("Goal"
+    :clause-processor
+    (my-clause-processor clause
+			 '( (:expand (foo1))
+			   (:python-file "test1")
+			   (:let ())
+			   (:hypothesize ()))))))
 
-;; ;; test2
-;; (defun foo2 (x) (+ x 3))
-;; (defun bar2 (y) (* 2 (foo2 y)))
+;; test2
+(defun foo2 (x) (+ x 3))
+(defun bar2 (y) (* 2 (foo2 y)))
 
-;; (defthm test2
-;;   (implies (and (and (rationalp y))
-;; 		(and (> y 1)))
-;; 	   (> (bar2 (foo2 y)) 12))
-;;   :hints
-;;   (("Goal"
-;;     :clause-processor
-;;     (my-clause-processor clause
-;; 			 '( (:expand (foo2 bar2))
-;; 			    (:python-file "test2")
-;; 			    (:let ())
-;; 			    (:hypothesize ()))))))
+(defthm test2
+  (implies (and (and (rationalp y))
+		(and (> y 1)))
+	   (> (bar2 (foo2 y)) 12))
+  :hints
+  (("Goal"
+    :clause-processor
+    (my-clause-processor clause
+			 '( (:expand (foo2 bar2))
+			    (:python-file "test2")
+			    (:let ())
+			    (:hypothesize ()))))))
 
-;; ;; test3
-;; (defun foo3 (x args) (+ x (nth 0 args) (nth 1 args)))
+;; test3
+(defun foo3 (x args) (+ x (nth 0 args) (nth 1 args)))
 
-;; (defthm test3
-;;   (implies (and (and (rationalp x)
-;; 		     (integerp i)
-;; 		     (integerp j))
-;; 		(and (> x 0)
-;; 		     (> i 0)
-;; 		     (> j 0)))
-;; 	   (> (foo3 x '(i j)) 0))
-;;   :hints
-;;   (("Goal"
-;;     :clause-processor
-;;     (my-clause-processor clause
-;; 			 '( (:expand (foo3))
-;; 			    (:python-file "test3")
-;; 			    (:let ())
-;; 			    (:hypothesize ()))))))
+(defthm test3
+  (implies (and (and (rationalp x)
+		     (integerp i)
+		     (integerp j))
+		(and (> x 0)
+		     (> i 0)
+		     (> j 0)))
+	   (> (foo3 x '(i j)) 0))
+  :hints
+  (("Goal"
+    :clause-processor
+    (my-clause-processor clause
+			 '( (:expand (foo3))
+			    (:python-file "test3")
+			    (:let ())
+			    (:hypothesize ()))))))
 
-;; ;; test4
-;; ;; x^2 + y^2 >= 2xy
-;; ;; a(x,y) = x*y
-;; ;; b(x) = 2*x = (a 2 x)
-;; ;; c(x,y) = x+y
-;; ;; d(x) = x^2 = (a x x)
-;; ;; e(x) = -x
-;; ;; f(x,y) = x-y = (c x -y) = (c x (e y))
-;; (defun a4 (x y) (* x y))
-;; (defun b4 (x) (a4 2 x))
-;; (defun c4 (x y) (+ x y))
-;; (defun d4 (x) (a4 x x))
-;; (defun e4 (x) (- x))
-;; (defun f4 (x y) (c4 x (e4 y)))
+;; test4
+;; x^2 + y^2 >= 2xy
+;; a(x,y) = x*y
+;; b(x) = 2*x = (a 2 x)
+;; c(x,y) = x+y
+;; d(x) = x^2 = (a x x)
+;; e(x) = -x
+;; f(x,y) = x-y = (c x -y) = (c x (e y))
+(defun a4 (x y) (* x y))
+(defun b4 (x) (a4 2 x))
+(defun c4 (x y) (+ x y))
+(defun d4 (x) (a4 x x))
+(defun e4 (x) (- x))
+(defun f4 (x y) (c4 x (e4 y)))
 
-;; (defthm test4
-;;     (implies (and (and (rationalp a)
-;; 		       (rationalp b))
-;; 		  (and))
-;; 	     (>= (f4 (d4 (c4 a b))
-;; 		     (a4 (b4 a) b))
-;; 		 (a4 (b4 a) b)))
-;;   :hints
-;;   (("Goal"
-;;     :clause-processor
-;;     (my-clause-processor clause
-;; 			 '( (:expand (a4 b4 c4 d4 e4 f4))
-;; 			    (:python-file "test4")
-;; 			    (:let ())
-;; 			    (:hypothesize ()))))))
+(defthm test4
+    (implies (and (and (rationalp a)
+		       (rationalp b))
+		  (and))
+	     (>= (f4 (d4 (c4 a b))
+		     (a4 (b4 a) b))
+		 (a4 (b4 a) b)))
+  :hints
+  (("Goal"
+    :clause-processor
+    (my-clause-processor clause
+			 '( (:expand (a4 b4 c4 d4 e4 f4))
+			    (:python-file "test4")
+			    (:let ())
+			    (:hypothesize ()))))))
 
 ;; ;; test5: with recursive call
 ;; ;; (fac)
